case_studies/tests/output/tests/proofs/proof_option_get_result.v
@@ -1,0 +1,39 @@
+From caesium Require Import lang notation.
+From refinedrust Require Import typing shims.
+From refinedrust.examples.tests.generated Require Import generated_code_tests generated_specs_tests generated_template_option_get_result.
+
+Set Default Proof Using "Type".
+
+Section proof.
+Context `{RRGS : !refinedrustGS Σ}.
+
+Lemma option_get_result_proof (π : thread_id) :
+  option_get_result_lemma π.
+Proof.
+  option_get_result_prelude.
+
+  rep <-! liRStep; liShow.
+
+  
+  (* Point: 
+     - I'm lacking the stratification instance, and we should totally add that.
+     - But if I move out, I won't be able to do that, and I need to handle that case.
+     - (Probably we shouldn't stratify that anyways. If we move stuff out, we cannot do that.)
+
+     Goal: we should just be able to deinit a bunch of stuff.
+      - we need to be careful to not do that if we could extract useful information.
+
+     Stratification before: get everything into shape and ensure invariants are upheld againn. 
+
+
+
+
+
+     
+    *)
+  all: print_remaining_goal.
+  Unshelve. all: sidecond_solver.
+  Unshelve. all: sidecond_hammer.
+  Unshelve. all: print_remaining_sidecond.
+Admitted.
+End proof.
