theories/rust_typing/mut_ref/place.v
@@ -22,7 +22,6 @@ Section place.
             (λ ltyi2 ri2, MutLtype (weak.(weak_lt) ltyi2 ri2) κ)
             (λ (r : place_rfn rti), PlaceIn (weak.(weak_rfn) r, γ))
             weak.(weak_R)) mstrong.(mstrong_weak))
-          None
           )))
     ⊢ typed_place π E L l (MutLtype lt2 κ) (PlaceIn (r, γ)) bmin0 (Owned wl) (DerefPCtx Na1Ord PtrOp true :: P) T.
   Proof.
@@ -40,7 +39,7 @@ Section place.
     iApply ("HR" with "[//] [//] [$LFT $TIME $LLCTX] HE HL [] Hb"). { iApply bor_kind_min_incl_l. }
     iModIntro. iIntros (L' κs l2 b2 bmin rti tyli ri [strong weak]) "#Hincl1 Hb Hs".
     iApply ("HΦ" $! _ _ _ _ bmin _ _ _ _ with "Hincl1 Hb").
-    simpl. iSplit; last iSplit.
+    simpl. iSplit.
     - (* strong *) iDestruct "Hs" as "[Hs _]".
       destruct strong as [ strong | ]; last done.
       iIntros (rti2 ltyi2 ri2) "Hl2 Hcond".
@@ -49,7 +48,7 @@ Section place.
       iFrame. iPureIntro. simp_ltypes. done.
     - (* weak *)
       destruct weak as [ weak | ]; last done.
-      iDestruct "Hs" as "(_ & Hs & _)".
+      iDestruct "Hs" as "(_ & Hs)".
       iIntros (ltyi2 ri2 bmin').
       iIntros "Hincl2 Hl2 Hcond".
       iMod ("Hs" with "Hincl2 Hl2 Hcond") as "(Hb & Hcond & $ & HR)".
@@ -59,7 +58,6 @@ Section place.
       iApply typed_place_cond_incl; last iApply "Hcond".
       + iApply bor_kind_min_incl_r.
       + iPureIntro. apply place_access_rt_rel_refl.
-    - done.
   Qed.
   Global Instance typed_place_mut_owned_inst {rto} E L π κ γ (lt2 : ltype rto) bmin0 r l wl P :
     TypedPlace E L π l (MutLtype lt2 κ) (#(r, γ)) bmin0 (Owned wl) (DerefPCtx Na1Ord PtrOp true :: P) | 30 := λ T, i2p (typed_place_mut_owned π κ lt2 P E L γ l r wl bmin0 T).
@@ -78,7 +76,6 @@ Section place.
               strong.(strong_R)) mstrong.(mstrong_strong))
             (* weak branch: just keep the MutLtype *)
             (fmap (λ weak, mk_weak (λ lti' ri', MutLtype (weak.(weak_lt) lti' ri') κ) (λ (r : place_rfn rti), #(weak.(weak_rfn) r, γ)) weak.(weak_R)) mstrong.(mstrong_weak))
-            None
             ))))
     ⊢ typed_place π E L l (MutLtype lt2 κ) #(r, γ) bmin0 (Uniq κ' γ') (DerefPCtx Na1Ord PtrOp true :: P) T.
   Proof.
@@ -101,7 +98,7 @@ Section place.
     iModIntro. iIntros (L'' κs' l2 b2 bmin rti tyli ri [strong weak]) "#Hincl1 Hb Hs".
     iApply ("HΦ" $! _ _ _ _ (Uniq κ' γ' ⊓ₖ bmin) _ _ _ _ with "[Hincl1] Hb").
     { iApply bor_kind_incl_trans; last iApply "Hincl1". iApply bor_kind_min_incl_r. }
-    simpl. iSplit; last iSplit.
+    simpl. iSplit.
     - (* strong update *)
       iDestruct "Hs" as "(Hs & _)". iDestruct "Hcl" as "(_ & Hcl)".
       destruct strong as [ strong | ]; last done.
@@ -114,7 +111,7 @@ Section place.
       iFrame. done.
     - (* weak update *)
       destruct weak as [ weak | ]; last done.
-      iDestruct "Hs" as "(_ & Hs & _)". iDestruct "Hcl" as "(Hcl & _)".
+      iDestruct "Hs" as "(_ & Hs)". iDestruct "Hcl" as "(Hcl & _)".
       iIntros (ltyi2 ri2 bmin') "#Hincl2 Hl2 Hcond".
       iMod ("Hs" with "[Hincl2] Hl2 Hcond") as "(Hb & Hcond & ? & HR)".
       { iApply bor_kind_incl_trans; first iApply "Hincl2". iApply bor_kind_min_incl_r. }
@@ -124,7 +121,6 @@ Section place.
       iModIntro. iFrame. rewrite llft_elt_toks_app. iFrame.
       iApply typed_place_cond_incl; last done.
       iApply bor_kind_min_incl_r.
-    - done.
   Qed.
   Global Instance typed_place_mut_uniq_inst {rto} E L π κ κ' γ γ' (lt2 : ltype rto) bmin0 r l P :
     TypedPlace E L π l (MutLtype lt2 κ) (#(r, γ)) bmin0 (Uniq κ' γ') (DerefPCtx Na1Ord PtrOp true :: P) | 30 := λ T, i2p (typed_place_mut_uniq π E L lt2 P l r κ γ κ' γ' bmin0 T).
@@ -144,7 +140,6 @@ Section place.
               (*strong.(strong_R)) strong)*)
             (* weak branch: just keep the MutLtype *)
             (fmap (λ weak, mk_weak (λ lti' ri', MutLtype (weak.(weak_lt) lti' ri') κ) (λ (r : place_rfn rti), #(weak.(weak_rfn) r, γ)) weak.(weak_R)) mstrong.(mstrong_weak))
-            None
             ))))
     ⊢ typed_place π E L l (MutLtype lt2 κ) #(r, γ) bmin0 (Shared κ') (DerefPCtx Na1Ord PtrOp true :: P) T.
   Proof.
@@ -166,12 +161,12 @@ Section place.
     iModIntro. iIntros (L'' κs' l2 b2 bmin rti tyli ri [strong weak]) "#Hincl1 Hb' Hs".
     iApply ("HΦ" $! _ _ _ _ (Shared κ' ⊓ₖ bmin) _ _ _ _ with "[Hincl1] Hb'").
     { iApply bor_kind_incl_trans; last iApply "Hincl1". iApply bor_kind_min_incl_r. }
-    simpl. iSplit; last iSplit.
+    simpl. iSplit.
     - (* strong update *)
       done.
     - (* weak update *)
       destruct weak as [ weak | ]; last done.
-      iDestruct "Hs" as "(_ & Hs & _)".
+      iDestruct "Hs" as "(_ & Hs)".
       iIntros (ltyi2 ri2 bmin') "#Hincl2 Hl2 Hcond".
       iMod ("Hs" with "[Hincl2] Hl2 Hcond") as "(Hb' & Hcond & ? & HR)".
       { iApply bor_kind_incl_trans; first iApply "Hincl2". iApply bor_kind_min_incl_r. }
@@ -183,7 +178,6 @@ Section place.
       + done.
       + iApply typed_place_cond_incl; last done.
         iApply bor_kind_min_incl_r.
-    - done.
   Qed.
   Global Instance typed_place_mut_shared_inst {rto} E L π κ κ' γ (lt2 : ltype rto) bmin0 r l P :
     TypedPlace E L π l (MutLtype lt2 κ) (#(r, γ)) bmin0 (Shared κ') (DerefPCtx Na1Ord PtrOp true :: P) | 30 := λ T, i2p (typed_place_mut_shared π E L lt2 P l r κ γ κ' bmin0 T).
