theories/rust_typing/struct/place.v
@@ -65,19 +65,6 @@ Section place.
     (*iApply typed_place_cond_rfn_refl.*)
   Qed.
 
-  (* needs to have lower priority than the id instance *)
-  Lemma typed_place_ofty_struct {rts} π E L l (tys : hlist type rts) (r : place_rfn (plist place_rfn rts)) sls bmin0 b P T :
-    typed_place π E L l (StructLtype (hmap (λ _, OfTy) tys) sls) r bmin0 b P T
-    ⊢ typed_place π E L l (◁ (struct_t sls tys)) r bmin0 b P T.
-  Proof.
-    iIntros "Hp". iApply typed_place_eqltype; last iFrame.
-    iIntros (?) "HL CTX HE".
-    iIntros (??). iApply struct_t_unfold.
-  Qed.
-  Global Instance typed_place_ofty_struct_inst {rts} π E L l (tys : hlist type rts) (r : place_rfn (plist place_rfn rts)) sls bmin0 b P :
-    TypedPlace E L π l (◁ (struct_t sls tys))%I r bmin0 b P | 30 :=
-        λ T, i2p (typed_place_ofty_struct π E L l tys r sls bmin0 b P T).
-
   Lemma typed_place_struct_owned {rts} (lts : hlist ltype rts) π E L (r : plist place_rfn rts) sls f wl bmin0 P l
     (T : place_cont_t (plist place_rfn rts)) :
     ((* sidecondition for other components *)
@@ -99,7 +86,6 @@ Section place.
             (λ lti2 ri2, StructLtype (hlist_insert_id (unit : Type) rts lts i (weak.(weak_lt) lti2 ri2)) sls)
             (λ (r' : place_rfn rti), #(plist_insert_id (unit : Type) rts r i (weak.(weak_rfn) r')))
             weak.(weak_R)) mstrong.(mstrong_weak))
-           None
           ))))
     ⊢ typed_place π E L l (StructLtype lts sls) (#r) bmin0 (Owned wl) (GetMemberPCtx sls f :: P) T.
   Proof.
@@ -134,7 +120,7 @@ Section place.
     { rewrite -Hlto -Hro. done. }
     iModIntro. iIntros (L' κs l2 b2 bmin rti ltyi ri [strong weak]) "#Hincl1 Hli Hcont".
     iApply ("HΦ" $! _ _ _ _ _ _ _ _ _ with "Hincl1 Hli").
-    simpl. iSplit; last iSplit.
+    simpl. iSplit.
     - (* strong *)
       destruct strong as [strong | ]; last done.
       iIntros (rti2 ltyi2 ri2) "Hli %Hst'".
@@ -149,7 +135,7 @@ Section place.
       iFrame. iPureIntro. done.
     - (* weak *)
       destruct weak as [ weak | ]; last done.
-      iDestruct "Hcont" as "(_ & Hcont & _)".
+      iDestruct "Hcont" as "(_ & Hcont)".
       iIntros (ltyi2 ri2 bmin') "#Hincl2 Hli Hcond".
       iMod ("Hcont" $! _ _ bmin' with "Hincl2 Hli Hcond") as "(Hb1 & Hcond & HL & HR)".
       simpl. iDestruct "Hc_close" as "[_ Hc_close]".
@@ -165,12 +151,9 @@ Section place.
       + iApply (struct_lift_place_cond_rfn_homo with "Hcond_rfn"); [done | lia].
       + iPureIntro. clear. induction rts; simpl; first done.
         constructor; first apply place_access_rt_rel_refl. done.
-    - (* immut *)
-      done.
   Qed.
-  Global Instance typed_place_struct_owned_inst π E L {rts} (lts : hlist ltype rts) (r : plist place_rfn rts) sls wl bmin0 f l P :
-    TypedPlace E L π l (StructLtype lts sls) (PlaceIn r) bmin0 (Owned wl) (GetMemberPCtx sls f :: P) | 30 :=
-        λ T, i2p (typed_place_struct_owned lts π E L r sls f wl bmin0 P l T).
+  Definition typed_place_struct_owned_inst := [instance @typed_place_struct_owned].
+  Global Existing Instance typed_place_struct_owned_inst | 30.
 
   Lemma typed_place_struct_uniq {rts} (lts : hlist ltype rts) π E L (r : plist place_rfn rts) sls f κ γ bmin0 P l
     (T : place_cont_t (plist place_rfn rts)) :
@@ -200,7 +183,6 @@ Section place.
             (λ lti2 ri2, StructLtype (hlist_insert_id (unit : Type) rts lts i (weak.(weak_lt) lti2 ri2)) sls)
             (λ (r' : place_rfn rti), #(plist_insert_id (unit : Type) rts r i (weak.(weak_rfn) r')))
             weak.(weak_R)) mstrong.(mstrong_weak))
-          None
           )))))
     ⊢ typed_place π E L l (StructLtype lts sls) (#r) bmin0 (Uniq κ γ) (GetMemberPCtx sls f :: P) T.
   Proof.
@@ -243,13 +225,13 @@ Section place.
     { rewrite -Hlto -Hro. done. }
     iModIntro. iIntros (L2 κs' l2 b2 bmin rti ltyi ri [strong weak]) "#Hincl1 Hli Hcont".
     iApply ("HΦ" $! _ _ _ _ _ _ _ _ _ with "Hincl1 Hli").
-    simpl. iSplit; last iSplit.
+    simpl. iSplit.
     - (* strong *)
       destruct strong as [strong | ]; last done.
       done.
     - (* weak *)
       destruct weak as [ weak | ]; last done.
-      iDestruct "Hcont" as "(_ & Hcont & _)".
+      iDestruct "Hcont" as "(_ & Hcont)".
       iIntros (ltyi2 ri2 bmin') "#Hincl2 Hli Hcond".
       iMod ("Hcont" $! _ _ bmin' with "Hincl2 Hli Hcond") as "(Hb1 & Hcond & HL & HR)".
       simpl. iDestruct "Hc_close" as "[_ Hc_close]".
@@ -266,11 +248,9 @@ Section place.
       rewrite llft_elt_toks_app. iFrame.
       iApply typed_place_cond_incl; last done.
       iApply bor_kind_min_incl_r.
-    - done.
   Qed.
-  Global Instance typed_place_struct_uniq_inst π E L {rts} (lts : hlist ltype rts) (r : plist place_rfn rts) sls κ γ bmin0 f l P :
-    TypedPlace E L π l (StructLtype lts sls) (PlaceIn r) bmin0 (Uniq κ γ) (GetMemberPCtx sls f :: P) | 30 :=
-        λ T, i2p (typed_place_struct_uniq lts π E L r sls f κ γ bmin0 P l T).
+  Definition typed_place_struct_uniq_inst := [instance @typed_place_struct_uniq].
+  Global Existing Instance typed_place_struct_uniq_inst | 30.
 
   Lemma typed_place_struct_shared {rts} (lts : hlist ltype rts) π E L (r : plist place_rfn rts) sls f κ bmin0 P l
     (T : place_cont_t (plist place_rfn rts)) :
@@ -295,7 +275,6 @@ Section place.
             (λ lti2 ri2, StructLtype (hlist_insert_id (unit : Type) rts lts i (weak.(weak_lt) lti2 ri2)) sls)
             (λ (r' : place_rfn rti), #(plist_insert_id (unit : Type) rts r i (weak.(weak_rfn) r')))
             weak.(weak_R)) mstrong.(mstrong_weak))
-          None
           ))))
     ⊢ typed_place π E L l (StructLtype lts sls) (#r) bmin0 (Shared κ) (GetMemberPCtx sls f :: P) T.
   Proof.
@@ -330,12 +309,12 @@ Section place.
     { rewrite -Hlto -Hro. done. }
     iIntros (L' κs l2 b2 bmin rti ltyi ri [strong weak]) "#Hincl1 Hli Hcont".
     iApply ("HΦ" $! _ _ _ _ _ _ _ _ _ with "Hincl1 Hli").
-    simpl. iSplit; last iSplit.
+    simpl. iSplit.
     - (* strong *)
       done.
     - (* weak *)
       destruct weak as [ weak | ]; last done.
-      iDestruct "Hcont" as "(_ & Hcont & _)".
+      iDestruct "Hcont" as "(_ & Hcont)".
       iIntros (ltyi2 ri2 bmin') "#Hincl2 Hli Hcond".
       iMod ("Hcont" $! _ _ bmin' with "Hincl2 Hli Hcond") as "(Hb1 & Hcond & HL & HR)".
       simpl. iDestruct "Hc_close" as "[_ Hc_close]".
@@ -351,12 +330,9 @@ Section place.
       + iApply (struct_lift_place_cond_rfn_homo with "Hcond_rfn"); [done | lia].
       + iPureIntro. clear. induction rts; simpl; first done.
         constructor; first apply place_access_rt_rel_refl. done.
-    - (* immut *)
-      done.
   Qed.
-  Global Instance typed_place_struct_shared_inst π E L {rts} (lts : hlist ltype rts) (r : plist place_rfn rts) sls κ bmin0 f l P :
-    TypedPlace E L π l (StructLtype lts sls) #r bmin0 (Shared κ) (GetMemberPCtx sls f :: P) | 30 :=
-        λ T, i2p (typed_place_struct_shared lts π E L r sls f κ bmin0 P l T).
+  Definition typed_place_struct_shared_inst := [instance @typed_place_struct_shared].
+  Global Existing Instance typed_place_struct_shared_inst | 30.
 
   (* TODO prove_place_cond *)
 End place.
